src/Spec/WpRefine.v
@@ -10,16 +10,16 @@ Section Dynamics.
   Context `(sem: Dynamics Op State).
   Notation proc := (proc Op).
   Notation step := sem.(step).
-  Notation exec := sem.(exec).
+  Notation exec := (exec sem).
 
   Context AState (absr: relation AState State unit).
   Context (wp: WPSetup sem).
 
   Theorem wp_refine T (p: proc T) (r: relation AState AState T) :
     (forall s s__a, absr s__a s tt ->
-             wp.(precond) p (fun v s' =>
-                               exists s__a', r s__a s__a' v /\
-                                      absr s__a' s' tt) s) ->
+             precond wp p (fun v s' =>
+                             exists s__a', r s__a s__a' v /\
+                                    absr s__a' s' tt) s) ->
     refines absr (exec p) r.
   Proof.
     intros.
